\chapter{test}
\section{العلاقة بين النوع الاول و النوع الثاني}
بما أن 
\[
T_n(x) = \cos(n \theta), \quad U_n(x) = \frac{\sin(n+1)\theta}{\sin\theta}
\]
فإن
\[
T_{n+1}(x) = \cos(n+1)\theta = \cos(n\theta)\cos\theta - \sin(n\theta)\sin\theta 
\]
\[
T_{n-1}(x) = \cos(n-1)\theta = \cos(n\theta)\cos\theta + \sin(n\theta)\sin\theta 
\]
و بالتالي
\[
T_{n-1}(x) - T_{n+1}(x) = 2 \sin(n\theta) \sin\theta = 2 \sin^2\theta \frac{\sin(n\theta)}{\sin\theta} 
\]
إذن 
\begin{equation}
	T_{n-1}(x) - T_{n+1}(x) = 2 (1-x^2) U_{n-1}(x) 
\end{equation}
بطرح المعادلتين (4) و (5) 
\[
U_{n+1}(x) - U_{n-1}(x) = \frac{2\sin\theta\cos(n+1)\theta}{\sin\theta} = 2 \cos(n+1)\theta
\]
إذن 
\begin{equation}
	U_{n+1}(x) - U_{n-1}(x)  = 2T_{n+1}(x)
\end{equation}
